theories/zoo_saturn/inf_mpmc_queue_2__opaque.v
@@ -1,7 +1,0 @@
-Require Import zoo_saturn.inf_mpmc_queue_2__code.
-
-#[global] Opaque inf_mpmc_queue_2٠create.
-#[global] Opaque inf_mpmc_queue_2٠size.
-#[global] Opaque inf_mpmc_queue_2٠is_empty.
-#[global] Opaque inf_mpmc_queue_2٠push.
-#[global] Opaque inf_mpmc_queue_2٠pop.
