theories/zoo_saturn/inf_queue_mpmc_2__opaque.v
@@ -1,0 +1,7 @@
+Require Import zoo_saturn.inf_queue_mpmc_2__code.
+
+#[global] Opaque inf_queue_mpmc_2٠create.
+#[global] Opaque inf_queue_mpmc_2٠size.
+#[global] Opaque inf_queue_mpmc_2٠is_empty.
+#[global] Opaque inf_queue_mpmc_2٠push.
+#[global] Opaque inf_queue_mpmc_2٠pop.
